add PdlRule, avoid List-paths, start PathIn defs

Pdl/Soundness.lean
@@ -124,7 +124,12 @@ inductive PathInLocal : ∀ {X}, LocalTableau X → Type
 | simEnd : PathInLocal (LocalTableau.sim _)
 
 inductive PathIn {H X} : ClosedTableau H X → Type
--- TODO  this would now have 8 cases, maybe first refactor `ClosedTableau`?
+-- TODO  this should now have 3 cases, after the refactor of `ClosedTableau` with separate `PdlRule`
+-- ClosedTableau.loc
+-- ClosedTableau.pdl
+-- ClosedTableau.rep
+
+def nodeAt : PathIn tab → TNode := sorry
 
 /-- The parent-child relation ◃ in a tableau -/
 def stepRel {H X} {ctX : ClosedTableau H X} : PathIn ctX → PathIn ctX → Prop
@@ -151,221 +156,26 @@ def K {H X} {ctX : ClosedTableau H X} : PathIn ctX → PathIn ctX → Prop
 def E {H X} {ctX : ClosedTableau H X} : PathIn ctX → PathIn ctX → Prop
 | t, s => (t ◃ s) ∨ K t s
 
--- Given:
--- - a local tableau (not necessarily a root)
--- - a path to be walked
--- return if succeeds: the TNode at the end of the path or a local end node and the remaining path
--- TOOD: rewrite with more match cases in term mode without "by"?
-def nodeInLocalAt (ltX : LocalTableau X) : List TNode → Option (TNode ⊕ (Subtype (fun Y => Y ∈ endNodesOf ltX) × List TNode))
-| [] => some (Sum.inl X) -- we have reached the destination
-| (Y::rest) => by
-    cases ltX
-    case byLocalRule B lnext lrApp =>
-      refine if Y_in : Y ∈ B then ?_ else ?_
-      · cases nodeInLocalAt (lnext Y Y_in) rest -- make a recursive call!
-        case none => exact none -- not found.
-        case some foo =>
-          cases foo
-          case inl Z =>
-            exact some (Sum.inl Z) -- found it!
-          case inr Z_ =>
-            rcases Z_ with ⟨⟨Z,Z_in⟩, remainder⟩
-            apply some
-            apply Sum.inr
-            refine ⟨⟨Z, ?_⟩, ?_⟩
-            · apply endNodeOfChild_to_endNode lrApp lnext rfl Y_in Z_in
-            · exact remainder
-      · exact none -- cannot follow path
-    case sim X_simp =>
-      apply some
-      apply Sum.inr
-      constructor
-      · use X
-        rw [endNodesOf, List.mem_singleton]
-      · exact Y::rest -- Problem: This case means "reminder" may be of same length still.
-
--- Given:
--- - a tableau (not necessarily a root)
--- - a path to be walked
--- return if succeeds: the TNode at the end of the path
-def nodeInAt : (Σ X HistX, ClosedTableau HistX X) → List TNode → Option TNode
-| ⟨X, hX, tab⟩, [] => some X -- we have reached the destination
-| ⟨X, hX, tab⟩, (Y::rest) => by
-      cases tab
-      case loc ltX next =>
-        cases nodeInLocalAt ltX (Y::rest)
-        case none => exact none
-        case some lt_res =>
-          cases lt_res
-          case inl Z => exact some Z -- reached end of path inside the local tableau.
-          case inr Y_end_remainder =>
-            rcases Y_end_remainder with ⟨⟨Y, Y_in⟩, remainder⟩
-            have : remainder.length < (Y::rest).length := sorry -- needed for termination, may need to add this in tabInLocalAt
-            exact nodeInAt ⟨Y, hX, next Y Y_in⟩ remainder
-      case mrkL =>
-        -- apply nodeInAt ?
-        sorry
-      case rep isRep =>
-        exact none -- fail, we cannot go to Y (and should be using Loopy from below!)
-      all_goals sorry
-termination_by
-   Xhtab toWalk => toWalk.length
-
--- Given:
--- - a local tableau (not necessarily a root)
--- - a path to be walked
--- return if succeeds: the local tableau at the end of the path or a local end node and the remaining path
--- TOOD: rewrite with more match cases in term mode without "by"?
-def tabInLocalAt (ltX : LocalTableau X) : List TNode → Option ((Σ Z, LocalTableau Z) ⊕ (Subtype (fun Y => Y ∈ endNodesOf ltX) × List TNode))
-| [] => some (Sum.inl ⟨X, ltX⟩) -- we have reached the destination
-| (Y::rest) => by
-    cases ltX
-    case byLocalRule B lnext lrApp =>
-      refine if Y_in : Y ∈ B then ?_ else ?_
-      · cases tabInLocalAt (lnext Y Y_in) rest -- make a recursive call!
-        case none => exact none -- not found.
-        case some foo =>
-          cases foo
-          case inl Z =>
-            exact some (Sum.inl Z) -- found it!
-          case inr Z_ =>
-            rcases Z_ with ⟨⟨Z,Z_in⟩, remainder⟩
-            apply some
-            apply Sum.inr
-            refine ⟨⟨Z, ?_⟩, ?_⟩
-            · apply endNodeOfChild_to_endNode lrApp lnext rfl Y_in Z_in
-            · exact remainder
-      · exact none -- cannot follow path
-    case sim X_simp =>
-      apply some
-      apply Sum.inr
-      constructor
-      · use X
-        rw [endNodesOf, List.mem_singleton]
-      · exact Y::rest -- Problem: This case means "reminder" may be of same length still.
-
--- Given:
--- - a tableau (not necessarily a root)
--- - a path to be walked
--- return if succeeds: the closed tableau at the end of the path
-def tabInAt : (Σ X HistX, ClosedTableau HistX X) → List TNode → Option (Σ Y HistY, ClosedTableau HistY Y)
-| ⟨X, hX, tab⟩, [] => some ⟨X, hX, tab⟩ -- we have reached the destination
-| ⟨X, hX, tab⟩, (Y::rest) => by
-      cases tab
-      case loc ltX next =>
-        cases tabInLocalAt ltX (Y::rest)
-        case none => exact none
-        case some lt_res =>
-          cases lt_res
-          case inl Z_ltZ =>
-            -- reached end of path inside the local tableau.
-            rcases Z_ltZ with ⟨Z, ltZ⟩
-            let ctZnext : (W : TNode) → W ∈ endNodesOf ltZ → ClosedTableau hX W :=
-              fun W W_in => next _ sorry -- Need: endNnodesOf ltZ ⊆ endNnodesOf ltX
-            let ctZ : ClosedTableau _ Z := ClosedTableau.loc ltZ ctZnext
-            exact some ⟨Z, _, ctZ⟩
-          case inr Y_end_remainder =>
-            rcases Y_end_remainder with ⟨⟨Y, Y_in⟩, remainder⟩
-            have : remainder.length < (Y::rest).length := sorry -- needed for termination, may need to add this in tabInLocalAt
-            exact tabInAt ⟨Y, hX, next Y Y_in⟩ remainder
-      case mrkL =>
-        -- apply tabInAt ?
-        sorry
-      case rep isRep =>
-        exact none -- fail, we cannot go to Y (and should be using Loopy from below!)
-      all_goals sorry
-termination_by
-   Xhtab toWalk => toWalk.length
-
--- Go one step, to Y, but possibly via a loop
--- Given:
--- - the root of a tableau
--- - a path already walked - needed to go back up to companion
--- - a path still to be walked
--- return: the tableau at the end of the path, possibly by looping via condition 6 repeats
---
--- IDEA: instead of using "tabInAt", add the Closed (or Local?!) tableau at "done" as another input?
-def goTo : (Σ R, ClosedTableau ([],[]) R) → List TNode → TNode → Option (Σ Y HistY, ClosedTableau HistY Y)
-| ⟨R, tab⟩, done, Y => by
-      cases tab_def : tabInAt ⟨R, ([],[]), tab⟩ done
-      case none =>
-        exact none -- this should never happen :-(
-      case some X_ =>
-        rcases X_ with ⟨X, HistX, ctX⟩
-        cases ctX
-        case loc ltX next =>
-          cases ltX
-          case byLocalRule B lnext lrApp =>
-            refine if Y_in : Y ∈ B then ?_ else ?_
-            -- move down a real step:
-            · let ltY := lnext Y Y_in
-              -- now need to turn ltY into a closed tableau. or change the return type?
-              let ctYnext : (Z : TNode) → Z ∈ endNodesOf ltY → ClosedTableau HistX Z :=
-                fun Z Z_in => next _ (endNodeOfChild_to_endNode lrApp lnext rfl Y_in Z_in)
-              let ctY : ClosedTableau _ Y := ClosedTableau.loc ltY ctYnext
-              exact some ⟨Y, _, ctY⟩
-            -- not found:
-            · exact none
-          case sim X_simp =>
-            have ctXnew := next X (by simp)
-            simp [endNodesOf, List.mem_singleton] at ctXnew
-            -- Now check that Y is among the successors given by non-local rules?
-            -- Or could we make a recursive call here?
-            -- Instead of `tabInAt ⟨R, ([],[]), tab⟩ done` above, now we want to consider ctXnew ?!
-            cases ctXnew
-            all_goals sorry
-        case mrkL =>
-          -- apply tabInAt ?
-          sorry
-        case rep theRep =>
-          simp only [condSixRepeat, List.any_eq_true] at theRep
-          rcases theRep with ⟨⟨k,Y⟩, getk, X_is_Y⟩ -- is k the index now? start with 0 or 1?
-          let (bef, aft) := HistX
-          -- now go back to the companion (and thus allow the path to be longer than the actual tableau)
-          let pathToCompanion : List TNode := done.drop (k+1) -- undo the steps since companion
-          have : pathToCompanion.length + 1 < done.length := by -- no more "rest" here as we only do one step
-            zify
-            -- ring -- why not working?
-            sorry
-          exact (tabInAt ⟨R, ([],[]), tab⟩ pathToCompanion)
-        all_goals sorry
-
--- MB: Lemma 7
 theorem loadedDiamondPaths
   {Root Δ : TNode}
   (tab : ClosedTableau ([],[]) Root) -- ensure History = [] here to prevent repeats from "above".
-  (path_to_Δ : List TNode)
-  (h : some tabΔ = tabInAt ⟨Root,_,tab⟩ path_to_Δ)
+  (path_to_Δ : PathIn tab)
+  (h : Δ = nodeAt path_to_Δ)
   {M : KripkeModel W} {v : W}
   (φ : AnyFormula)
   (negLoad_in : NegLoadFormula_in_TNode (~'⌊α⌋φ) Δ) -- FIXME: ∈ not working here?
   (v_X : (M,v) ⊨ Δ)
   (v_α_w : relate M α v w)
   (w_φ : (M,w) ⊨ ~''φ)
-  : ∃ path_Δ_to_Γ : List TNode,
-    ∃ Γ ∈ tabInAt ⟨Root,_,tab⟩ (path_to_Δ ++ path_Δ_to_Γ),
-    (AnyNegFormula_in_TNode (~''φ) Γ.1) -- FIXME: ∈ not working here?
-    ∧
-    (M,w) ⊨ Γ.1 :=
+  : ∃ Γ : TNode,
+    ∃ path_to_Γ : PathIn tab,
+        Γ = nodeAt path_to_Γ
+      -- TODO: must be an extension of path_to_Δ
+      ∧ (AnyNegFormula_in_TNode (~''φ) Γ) -- FIXME: ∈ not working here?
+      ∧ (M,w) ⊨ Γ :=
   by
   let ⟨L,R,O⟩ := Δ
-  let ⟨ΔNode, ΔHist, ΔTab⟩ := tabΔ
-  -- cases tab -- No, we want to distinguish by cases what is happening at Δ
-  cases ΔTab
-  case mrkL =>
-    -- it should be impossible to apply (M+)
-    -- because we already have a loaded formula in Δ
-    simp at negLoad_in
-    cases negLoad_in
-    case inl hyp => subst hyp; sorry
-    all_goals sorry
-
   all_goals sorry
-
--- MB: Lemma 8
--- theorem freeSatDown : Prop := sorry
--- have := localRuleTruth
--- have := loadedDiamondPaths
 
 
 theorem tableauThenNotSat : ∀ X, ClosedTableau LoadHistory.nil X → ¬satisfiable X :=
@@ -373,7 +183,7 @@ theorem tableauThenNotSat : ∀ X, ClosedTableau LoadHistory.nil X → ¬satisfi
   intro X t
   sorry
 
--- Theorem 2, page 30
+
 theorem correctness : ∀LR : TNode, satisfiable LR → consistent LR :=
   by
     intro LR
